isabelle/Testing.thy
@@ -11,6 +11,8 @@ definition test_parser :: "'a Parser \<Rightarrow> string \<Rightarrow> 'a Parse
     LR_Success result \<Rightarrow> run_parser p ''Test.b'' result
     | LR_Error loc \<Rightarrow> PR_Error loc)"
 
-value "lex ''Test.b'' ''0x10000000000000000''"
+(* value "lex ''Test.b'' ''0x10000000000000000''" *)
 
-value "test_parser (parse_module) ''module Foo interface { const x: i32 = 1000; }''"
+(* value "test_parser (parse_term) ''1''" *)
+
+value "test_parser (parse_module) ''module MRange2 interface {} function test() { assume 1 ; }''"
